Simplify the model of mutexes by removing the exclusive token.

theories/lang/lib/lock.v
@@ -15,42 +15,24 @@ Definition release : val := λ: ["l"], "l" <-ˢᶜ #false.
    protocol into shared borrows.  Cancellable invariants don't work because
    their cancelling view shift has a non-empty mask, and it would have to be
    executed in the consequence view shift of a borrow. *)
-
-(** The CMRA we need. *)
-(* Not bundling heapG, as it may be shared with other users. *)
-Class lockG Σ := LockG { lock_tokG :> inG Σ (exclR unitC) }.
-Definition lockΣ : gFunctors := #[GFunctor (exclR unitC)].
-
-Instance subG_lockΣ {Σ} : subG lockΣ Σ → lockG Σ.
-Proof. solve_inG. Qed.
-
 Section proof.
-  Context `{!lrustG Σ, !lockG Σ}.
+  Context `{!lrustG Σ}.
 
-  Definition lock_proto (γ : gname) (l : loc) (R : iProp Σ) : iProp Σ :=
-    (∃ b : bool, l ↦ #b ∗ if b then True else own γ (Excl ()) ∗ R)%I.
+  Definition lock_proto (l : loc) (R : iProp Σ) : iProp Σ :=
+    (∃ b : bool, l ↦ #b ∗ if b then True else R)%I.
 
-  Definition locked (γ : gname): iProp Σ := own γ (Excl ()).
-
-  Global Instance lock_proto_ne γ l : NonExpansive (lock_proto γ l).
+  Global Instance lock_proto_ne l : NonExpansive (lock_proto l).
   Proof. solve_proper. Qed.
 
-  Global Instance locked_timeless γ : TimelessP (locked γ).
-  Proof. apply _. Qed.
-
-  Lemma locked_exclusive (γ : gname) : locked γ -∗ locked γ -∗ False.
-  Proof. iIntros "H1 H2". by iDestruct (own_valid_2 with "H1 H2") as %?. Qed.
-
-  Lemma lock_proto_iff γ l R R' :
-    □ (R ↔ R') -∗ lock_proto γ l R -∗ lock_proto γ l R'.
+  Lemma lock_proto_iff l R R' :
+    □ (R ↔ R') -∗ lock_proto l R -∗ lock_proto l R'.
   Proof.
     iIntros "#HRR' Hlck". iDestruct "Hlck" as (b) "[Hl HR]". iExists b.
-    iFrame "Hl". destruct b; first done. iDestruct "HR" as "[$ HR]".
-    by iApply "HRR'".
+    iFrame "Hl". destruct b; first done. by iApply "HRR'".
   Qed.
 
-  Lemma lock_proto_iff_proper γ l R R' :
-    □ (R ↔ R') -∗ □ (lock_proto γ l R ↔ lock_proto γ l R').
+  Lemma lock_proto_iff_proper l R R' :
+    □ (R ↔ R') -∗ □ (lock_proto l R ↔ lock_proto l R').
   Proof.
     iIntros "#HR !#". iSplit; iIntros "Hlck"; iApply (lock_proto_iff with "[HR] Hlck").
     - done.
@@ -59,43 +41,39 @@ Section proof.
 
   (** The main proofs. *)
   Lemma lock_proto_create (R : iProp Σ) l (b : bool) :
-    l ↦ #b -∗ (if b then True else ▷ R) ==∗ ∃ γ, ▷ lock_proto γ l R.
+    l ↦ #b -∗ (if b then True else ▷ R) ==∗ ▷ lock_proto l R.
   Proof.
-    iIntros "Hl HR".
-    iMod (own_alloc (Excl ())) as (γ) "Hγ"; first done.
-    iExists _, _. iFrame "Hl". destruct b; first done. by iFrame.
+    iIntros "Hl HR". iExists _. iFrame "Hl". destruct b; first done. by iFrame.
   Qed.
 
-  Lemma lock_proto_destroy γ l R :
-    lock_proto γ l R -∗ ∃ (b : bool), l ↦ #b ∗ if b then True else R.
+  Lemma lock_proto_destroy l R :
+    lock_proto l R -∗ ∃ (b : bool), l ↦ #b ∗ if b then True else R.
   Proof.
-    iIntros "Hlck". iDestruct "Hlck" as (b) "[Hl HR]".
-    iExists b. iFrame "Hl". destruct b; first done.
-    iDestruct "HR" as "[_ $]".
+    iIntros "Hlck". iDestruct "Hlck" as (b) "[Hl HR]". auto with iFrame.
   Qed.
 
   Lemma mklock_unlocked_spec (R : iProp Σ) (l : loc) v :
-    {{{ l ↦ v ∗ ▷ R }}} mklock_unlocked [ #l ] {{{ γ, RET #(); ▷ lock_proto γ l R }}}.
+    {{{ l ↦ v ∗ ▷ R }}} mklock_unlocked [ #l ] {{{ RET #(); ▷ lock_proto l R }}}.
   Proof.
     iIntros (Φ) "[Hl HR] HΦ". wp_lam. rewrite -wp_fupd. wp_write.
-    iMod (lock_proto_create with "Hl HR") as (γ) "Hproto".
+    iMod (lock_proto_create with "Hl HR") as "Hproto".
     iApply "HΦ". by iFrame.
   Qed.
 
   Lemma mklock_locked_spec (R : iProp Σ) (l : loc) v :
-    {{{ l ↦ v }}} mklock_locked [ #l ] {{{ γ, RET #(); ▷ lock_proto γ l R }}}.
+    {{{ l ↦ v }}} mklock_locked [ #l ] {{{ RET #(); ▷ lock_proto l R }}}.
   Proof.
     iIntros (Φ) "Hl HΦ". wp_lam. rewrite -wp_fupd. wp_write.
-    iMod (lock_proto_create with "Hl [//]") as (γ) "Hproto".
+    iMod (lock_proto_create with "Hl [//]") as "Hproto".
     iApply "HΦ". by iFrame.
   Qed.
 
   (* At this point, it'd be really nice to have some sugar for symmetric
      accessors. *)
-  Lemma try_acquire_spec E γ l R P :
-    □ (P ={E,∅}=∗ ▷ lock_proto γ l R ∗ (▷ lock_proto γ l R ={∅,E}=∗ P)) -∗
+  Lemma try_acquire_spec E l R P :
+    □ (P ={E,∅}=∗ ▷ lock_proto l R ∗ (▷ lock_proto l R ={∅,E}=∗ P)) -∗
     {{{ P }}} try_acquire [ #l ] @ E
-    {{{ b, RET #b; (if b is true then locked γ ∗ ▷ R else True) ∗ P }}}.
+    {{{ b, RET #b; (if b is true then ▷ R else True) ∗ P }}}.
   Proof.
     iIntros "#Hproto !# * HP HΦ".
     wp_rec. iMod ("Hproto" with "HP") as "(Hinv & Hclose)".
@@ -104,30 +82,29 @@ Section proof.
       iMod ("Hclose" with "[Hl]"); first (iExists true; by eauto).
       iModIntro. iApply ("HΦ" $! false). auto.
     - wp_apply (wp_cas_int_suc with "Hl"); [done..|]. iIntros "Hl".
-      iDestruct "HR" as "[Hγ HR]".
       iMod ("Hclose" with "[Hl]") as "HP"; first (iExists true; by eauto).
-      iModIntro. rewrite /locked. iApply ("HΦ" $! true with "[$Hγ $HR $HP]").
+      iModIntro. iApply ("HΦ" $! true); iFrame.
   Qed.
 
-  Lemma acquire_spec E γ l R P :
-    □ (P ={E,∅}=∗ ▷ lock_proto γ l R ∗ (▷ lock_proto γ l R ={∅,E}=∗ P)) -∗
-    {{{ P }}} acquire [ #l ] @ E {{{ RET #(); locked γ ∗ ▷ R ∗ P }}}.
+  Lemma acquire_spec E l R P :
+    □ (P ={E,∅}=∗ ▷ lock_proto l R ∗ (▷ lock_proto l R ={∅,E}=∗ P)) -∗
+    {{{ P }}} acquire [ #l ] @ E {{{ RET #(); ▷ R ∗ P }}}.
   Proof.
     iIntros "#Hproto !# * HP HΦ". iLöb as "IH". wp_rec.
     wp_apply (try_acquire_spec with "Hproto HP"). iIntros ([]).
-    - iIntros "[[Hlked HR] Hown]". wp_if. iApply "HΦ"; iFrame.
+    - iIntros "[HR Hown]". wp_if. iApply "HΦ"; iFrame.
     - iIntros "[_ Hown]". wp_if. iApply ("IH" with "Hown HΦ").
   Qed.
 
-  Lemma release_spec E γ l R P :
-    □ (P ={E,∅}=∗ ▷ lock_proto γ l R ∗ (▷ lock_proto γ l R ={∅,E}=∗ P)) -∗
-    {{{ locked γ ∗ R ∗ P }}} release [ #l ] @ E {{{ RET #(); P }}}.
+  Lemma release_spec E l R P :
+    □ (P ={E,∅}=∗ ▷ lock_proto l R ∗ (▷ lock_proto l R ={∅,E}=∗ P)) -∗
+    {{{ R ∗ P }}} release [ #l ] @ E {{{ RET #(); P }}}.
   Proof.
-    iIntros "#Hproto !# * (Hlocked & HR & HP) HΦ". wp_let.
+    iIntros "#Hproto !# * (HR & HP) HΦ". wp_let.
     iMod ("Hproto" with "HP") as "(Hinv & Hclose)".
     iDestruct "Hinv" as (b) "[? _]". wp_write. iApply "HΦ".
     iApply "Hclose". iExists false. by iFrame.
   Qed.
 End proof.
 
-Typeclasses Opaque lock_proto locked.
+Typeclasses Opaque lock_proto.
